reflection: TermEq: termination proven, only issues from 2908 remain

ulib/FStar.Reflection.TermEq.fst
@@ -10,12 +10,17 @@ let rec allP0 #a (pred : a -> Type0) (l : list a) : Type0 =
   | [] -> True
   | x::xs -> pred x /\ allP0 pred xs
 
-let rec allP #a #b (top:b) (pred : (x:a{x << top}) -> Type0) (l : list a{l << top}) : Type0 =
+let rec allP #a #b (top:b) (pred : (x:a{x << top}) -> Type0) (l : list a{l << top \/ l === top}) : Type0 =
   match l with
   | [] -> True
   | x::xs -> pred x /\ allP top pred xs
 
-let optP #a (pred : a -> Type0) (o : option a) : Type0 =
+let optP0 #a (pred : a -> Type0) (o : option a) : Type0 =
+  match o with
+  | None -> True
+  | Some x -> pred x
+  
+let optP #a #b (top:b) (pred : (x:a{x << top}) -> Type0) (o : option a{o << top}) : Type0 =
   match o with
   | None -> True
   | Some x -> pred x
@@ -116,27 +121,35 @@ let rec list_eq #a cmp l1 l2 =
 
 val list_dec_eq :
 #a:Type u#aa -> #b:Type u#bb -> top1:b -> top2:b ->
-  f:(x:a{x << top1} -> y:a{y << top2} -> cmpres x y) ->
-  l1:(list a){l1 << top1} -> l2:(list a){l2 << top2} ->
+  f:(x:a -> y:a{x << top1 /\ y << top2} -> cmpres x y) ->
+  l1:(list a) -> l2:(list a){l1 << top1 /\ l2 << top2} ->
   cmpres l1 l2
 let rec list_dec_eq #a top1 top2 cmp l1 l2 =
   match l1, l2 with
   | [], [] -> Eq
-  | x::xs, y::ys ->
-    cmp x y &&& list_dec_eq top1 top2 cmp xs ys
+  | x::xs, y::ys -> cmp x y &&& list_dec_eq top1 top2 cmp xs ys
   | _ -> Neq
 
-(* Refinements shaped differently *)
-val list_dec_eq2 :
-#a:Type u#aa -> #b:Type u#bb -> top1:b -> top2:b ->
-  f:(x:a -> y:a{x << top1 /\ y << top2} -> cmpres x y) ->
-  l1:(list a){l1 << top1} -> l2:(list a){l2 << top2} ->
-  cmpres l1 l2
-let rec list_dec_eq2 #a top1 top2 cmp l1 l2 =
-  match l1, l2 with
-  | [], [] -> Eq
-  | x::xs, y::ys ->
-    cmp x y &&& list_dec_eq2 top1 top2 cmp xs ys
+val opt_dec_eq : #a:Type -> #b:Type -> top1:b -> top2:b ->
+  (f : (x:a -> y:a{x << top1 /\ y << top2} -> cmpres x y)) ->
+  o1:(option a){o1 << top1} -> o2:(option a){o2 << top2} ->
+  cmpres o1 o2
+let opt_dec_eq top1 top2 cmp o1 o2 =
+  match o1, o2 with
+  | None, None -> Eq
+  | Some x, Some y -> cmp x y
+  | _ -> Neq
+
+val either_dec_eq : #a:Type -> #b:Type -> #c:Type -> top1:c -> top2:c ->
+  (x:a -> y:a{x<<top1 /\ y<<top2} -> cmpres x y) ->
+  (x:b -> y:b{x<<top1 /\ y<<top2} -> cmpres x y) ->
+  e1 :(either a b){e1 << top1} ->
+  e2 :(either a b){e2 << top2} ->
+  cmpres e1 e2
+let either_dec_eq top1 top2 cmpa cmpb e1 e2 =
+  match e1, e2 with
+  | Inl x, Inl y -> cmpa x y
+  | Inr x, Inr y -> cmpb x y
   | _ -> Neq
 
 val eq_eq : #a:eqtype -> comparator_for a
@@ -152,9 +165,8 @@ let ident_eq i1 i2 =
   Sealed.sealed_singl (snd i1) (snd i2);
   eq_eq (fst i1) (fst i2)
 
-val univ_eq         : comparator_for universe
-
-let rec univ_eq (u1 u2 : universe) : cmpres u1 u2 =
+val univ_eq : comparator_for universe
+let rec univ_eq (u1 u2 : universe) =
   pack_inspect_universe u1;
   pack_inspect_universe u2;
   let uv1 = inspect_universe u1 in
@@ -162,13 +174,11 @@ let rec univ_eq (u1 u2 : universe) : cmpres u1 u2 =
   match uv1, uv2 with
   | Uv_Zero, Uv_Zero -> Eq
   | Uv_Succ u1, Uv_Succ u2 -> univ_eq u1 u2
-  | Uv_Max us1, Uv_Max us2 ->
-    list_dec_eq2 u1 u2 univ_eq us1 us2
+  | Uv_Max us1, Uv_Max us2 -> list_dec_eq u1 u2 univ_eq us1 us2
   | Uv_BVar v1, Uv_BVar v2 -> eq_eq v1 v2
   | Uv_Name n1, Uv_Name n2 -> ident_eq n1 n2
   | Uv_Unif u1, Uv_Unif u2 -> Unknown
   | Uv_Unk, Uv_Unk -> Eq
-
   | _ -> Neq
 
 val const_eq : comparator_for vconst
@@ -199,7 +209,6 @@ val pat_arg_eq      : comparator_for (pattern & bool)
 val br_eq           : comparator_for branch
 val match_returns_ascription_eq : comparator_for match_returns_ascription
 
-[@@admit_termination]
 let rec term_eq t1 t2 =
   pack_inspect_inv t1;
   pack_inspect_inv t2;
@@ -212,7 +221,7 @@ let rec term_eq t1 t2 =
   | Tv_BVar v1, Tv_BVar v2 -> bv_eq v1 v2
   | Tv_FVar f1, Tv_FVar f2 -> fv_eq f1 f2
   | Tv_UInst f1 u1, Tv_UInst f2 u2 ->
-    fv_eq f1 f2 &&& list_dec_eq2 t1 t2 univ_eq u1 u2
+    fv_eq f1 f2 &&& list_dec_eq t1 t2 univ_eq u1 u2
 
   | Tv_App h1 a1, Tv_App h2 a2 ->
     term_eq h1 h2 &&& arg_eq a1 a2
@@ -241,7 +250,7 @@ let rec term_eq t1 t2 =
 
   | Tv_Let r1 attrs1 bv1 ty1 e1 b1, Tv_Let r2 attrs2 bv2 ty2 e2 b2 ->
     eq_eq r1 r2
-     &&& list_eq term_eq attrs1 attrs2
+     &&& list_dec_eq t1 t2 term_eq attrs1 attrs2
      &&& binding_bv_eq bv1 bv2
      &&& term_eq ty1 ty2
      &&& term_eq e1 e2
@@ -249,19 +258,19 @@ let rec term_eq t1 t2 =
 
   | Tv_Match sc1 o1 brs1, Tv_Match sc2 o2 brs2 ->
     term_eq sc1 sc2
-     &&& opt_eq match_returns_ascription_eq o1 o2
-     &&& list_eq br_eq brs1 brs2
+     &&& opt_dec_eq t1 t2 match_returns_ascription_eq o1 o2
+     &&& list_dec_eq t1 t2 br_eq brs1 brs2
 
-  | Tv_AscribedT e1 t1 tacopt1 eq1, Tv_AscribedT e2 t2 tacopt2 eq2 ->
+  | Tv_AscribedT e1 ta1 tacopt1 eq1, Tv_AscribedT e2 ta2 tacopt2 eq2 ->
     term_eq e1 e2
-     &&& term_eq t1 t2
-     &&& opt_eq term_eq tacopt1 tacopt2
+     &&& term_eq ta1 ta2
+     &&& opt_dec_eq t1 t2 term_eq tacopt1 tacopt2
      &&& eq_eq eq1 eq2
 
   | Tv_AscribedC e1 c1 tacopt1 eq1, Tv_AscribedC e2 c2 tacopt2 eq2 ->
     term_eq e1 e2
      &&& comp_eq c1 c2
-     &&& opt_eq term_eq tacopt1 tacopt2
+     &&& opt_dec_eq t1 t2 term_eq tacopt1 tacopt2
      &&& eq_eq eq1 eq2
 
   | Tv_Unknown, Tv_Unknown -> Eq
@@ -287,10 +296,12 @@ and binding_bv_eq x1 x2 =
    then Eq
    else Neq
 
-and match_returns_ascription_eq (b1, (tc1, tacopt1, eq1)) (b2, (tc2, tacopt2, eq2)) =
+and match_returns_ascription_eq asc1 asc2 =
+  let (b1, (tc1, tacopt1, eq1)) = asc1 in
+  let (b2, (tc2, tacopt2, eq2)) = asc2 in
   binder_eq b1 b2
-   &&& either_eq term_eq comp_eq tc1 tc2
-   &&& opt_eq term_eq tacopt1 tacopt2
+   &&& either_dec_eq asc1 asc2 term_eq comp_eq tc1 tc2
+   &&& opt_dec_eq asc1 asc2 term_eq tacopt1 tacopt2
    &&& eq_eq eq1 eq2
 
 and binder_eq b1 b2 =
@@ -301,7 +312,7 @@ and binder_eq b1 b2 =
   binding_bv_eq bv1.binder_bv bv2.binder_bv
    &&& term_eq bv1.binder_sort bv2.binder_sort
    &&& aqual_eq bv1.binder_qual bv2.binder_qual
-   &&& list_eq term_eq bv1.binder_attrs bv2.binder_attrs
+   &&& list_dec_eq b1 b2 term_eq bv1.binder_attrs bv2.binder_attrs
 
 and comp_eq c1 c2 =
   let cv1 = inspect_comp c1 in
@@ -319,15 +330,17 @@ and comp_eq c1 c2 =
      &&& term_eq pat1 pat2
 
   | C_Eff us1 ef1 t1 args1 dec1, C_Eff us2 ef2 t2 args2 dec2 ->
-    list_eq univ_eq us1 us2
+    list_dec_eq c1 c2 univ_eq us1 us2
      &&& eq_eq ef1 ef2
      &&& term_eq t1 t2
-     &&& list_eq arg_eq args1 args2
-     &&& list_eq term_eq dec1 dec2
+     &&& list_dec_eq c1 c2 arg_eq args1 args2
+     &&& list_dec_eq c1 c2 term_eq dec1 dec2
 
   | _ -> Neq
 
-and br_eq br1 br2 = pair_eq pat_eq term_eq br1 br2
+and br_eq br1 br2 =
+  //pair_eq pat_eq term_eq br1 br2
+  pat_eq (fst br1) (fst br2) &&& term_eq (snd br1) (snd br2)
 
 and pat_eq p1 p2 =
   match p1, p2 with
@@ -335,11 +348,13 @@ and pat_eq p1 p2 =
     Sealed.sealed_singl st1 st2;
     bv_eq v1 v2
   | Pat_Constant c1, Pat_Constant c2 -> const_eq c1 c2
-  | Pat_Dot_Term t1, Pat_Dot_Term t2 -> opt_eq term_eq t1 t2
+  | Pat_Dot_Term t1, Pat_Dot_Term t2 -> opt_dec_eq p1 p2 term_eq t1 t2
   | Pat_Cons f1 us1 args1, Pat_Cons f2 us2 args2 ->
+    assert (us1 << p1);
+    assert (us2 << p2);
     fv_eq f1 f2
-     &&& opt_eq (list_eq univ_eq) us1 us2
-     &&& list_eq pat_arg_eq args1 args2
+     &&& opt_dec_eq p1 p2 (list_dec_eq p1 p2 univ_eq) us1 us2
+     &&& list_dec_eq p1 p2 pat_arg_eq args1 args2
 
   | _ -> Neq
 
@@ -360,7 +375,7 @@ let rec defined_list #a (f : comparator_for a) (l1 l2 : list a)
 let rec defined_list_dec #a #b (t1 t2 : b) (f : comparator_for a)
   (l1 : list a{l1 << t1})
   (l2 : list a{l2 << t2})
-  : Lemma (requires (def2 f l1 l2)) (ensures defined (list_dec_eq2 t1 t2 f l1 l2))
+  : Lemma (requires (def2 f l1 l2)) (ensures defined (list_dec_eq t1 t2 f l1 l2))
   = match l1, l2 with
     | [], [] -> ()
     | x::xs, y::ys -> defined_list_dec t1 t2 f xs ys
@@ -388,7 +403,7 @@ let rec univ_faithful_lemma (u1 u2 : universe) =
     assert_norm (faithful_univ u1 <==> allP u1 faithful_univ us1); // #2908
     assert_norm (faithful_univ u2 <==> allP u2 faithful_univ us2); // #2908
     univ_faithful_lemma_list u1 u2 us1 us2;
-    assert_norm (univ_eq u1 u2 == list_dec_eq2 u1 u2 univ_eq us1 us2); // #2908
+    assert_norm (univ_eq u1 u2 == list_dec_eq u1 u2 univ_eq us1 us2); // #2908
     ()
   | Uv_BVar _, Uv_BVar _ -> ()
   | Uv_Name _, Uv_Name _ -> ()
@@ -396,7 +411,7 @@ let rec univ_faithful_lemma (u1 u2 : universe) =
 
 and univ_faithful_lemma_list #b (u1 u2 : b) (us1 : list universe{us1 << u1}) (us2 : list universe{us2 << u2})
   : Lemma (requires allP u1 faithful_univ us1 /\ allP u2 faithful_univ us2)
-          (ensures defined (list_dec_eq2 u1 u2 univ_eq us1 us2))
+          (ensures defined (list_dec_eq u1 u2 univ_eq us1 us2))
           (decreases us1)
   =
     introduce forall x y. L.memP x us1 /\ L.memP y us2 ==> defined (univ_eq x y) with
@@ -410,7 +425,6 @@ and univ_faithful_lemma_list #b (u1 u2 : b) (us1 : list universe{us1 << u1}) (us
     defined_list_dec u1 u2 univ_eq us1 us2
 
 val faithful : term -> Type0
-[@@admit_termination]
 let rec faithful t =
   match inspect_ln t with
   | Tv_Var _
@@ -445,17 +459,17 @@ let rec faithful t =
   | Tv_Match sc o brs ->
     faithful sc
      /\ None? o // stopgap
-     /\ allP0 faithful_branch brs
+     /\ allP t faithful_branch brs
 
-  | Tv_AscribedT e t tacopt eq ->
+  | Tv_AscribedT e ta tacopt eq ->
     faithful e
-     /\ faithful t
-     /\ optP faithful tacopt
+     /\ faithful ta
+     /\ optP t faithful tacopt
 
   | Tv_AscribedC e c tacopt eq ->
     faithful e
      /\ faithful_comp c
-     /\ optP faithful tacopt
+     /\ optP t faithful tacopt
 
 and faithful_arg (a : argv) : Type0 =
   faithful (fst a) /\ faithful_qual (snd a)
@@ -479,17 +493,18 @@ and faithful_pattern (p : pattern) : Type0 =
   match p with
   | Pat_Constant _ -> True
   | Pat_Cons h usopt pats ->
-    optP (allP0 faithful_univ) usopt
-     /\ allP0 faithful_pattern_arg pats
+    optP p (allP p faithful_univ) usopt
+     /\ allP p faithful_pattern_arg pats
   (* non-binding bvs are always OK *)
   | Pat_Var bv _ -> True
   | Pat_Dot_Term None -> True
   | Pat_Dot_Term (Some t) -> faithful t
 
-and faithful_pattern_arg (pb : pattern * bool) =
+and faithful_pattern_arg (pb : pattern * bool) : Type0 =
   faithful_pattern (fst pb)
 
-and faithful_attrs ats = allP0 faithful ats
+and faithful_attrs ats : Type0 =
+  allP ats faithful ats
 
 and faithful_comp c =
   match inspect_comp c with
@@ -497,16 +512,15 @@ and faithful_comp c =
   | C_GTotal t -> faithful t
   | C_Lemma pre post pats -> faithful pre /\ faithful post /\ faithful pats
   | C_Eff us ef r args decs ->
-    allP0 faithful_univ us
+    allP c faithful_univ us
      /\ faithful r
-     /\ allP0 faithful_arg args
-     /\ allP0 faithful decs
+     /\ allP c faithful_arg args
+     /\ allP c faithful decs
 
 val faithful_lemma (t1:term) (t2:term) : Lemma (requires faithful t1 /\ faithful t2) (ensures defined (term_eq t1 t2))
 
 #push-options "--z3rlimit 40"
 
-[@@admit_termination]
 let rec faithful_lemma (t1 t2 : term) =
   match inspect_ln t1, inspect_ln t2 with
   | Tv_Var _, Tv_Var _
@@ -522,7 +536,7 @@ let rec faithful_lemma (t1 t2 : term) =
     assert_norm (allP t1 faithful_univ us1);
     assert_norm (allP t2 faithful_univ us2);
     univ_faithful_lemma_list t1 t2 us1 us2;
-    assert_norm (term_eq t1 t2 == (fv_eq f1 f2 &&& list_dec_eq2 t1 t2 univ_eq us1 us2));
+    assert_norm (term_eq t1 t2 == (fv_eq f1 f2 &&& list_dec_eq t1 t2 univ_eq us1 us2));
     ()
 
   | Tv_Const c1, Tv_Const c2 -> ()
@@ -542,13 +556,15 @@ let rec faithful_lemma (t1 t2 : term) =
     faithful_lemma t1 t2
 
   | Tv_Let r1 ats1 x1 ty1 e1 b1, Tv_Let r2 ats2 x2 ty2 e2 b2 ->
-    faithful_lemma_attrs ats1 ats2;
+    assume (faithful t1 ==> faithful_attrs ats1); //2908
+    assume (faithful t2 ==> faithful_attrs ats2); //2908
+    faithful_lemma_attrs_dec t1 t2 ats1 ats2;
     faithful_lemma ty1 ty2;
     faithful_lemma e1 e2;
     faithful_lemma b1 b2;
     assume (
      (eq_eq r1 r2
-     &&& list_eq term_eq ats1 ats2
+     &&& list_dec_eq t1 t2 term_eq ats1 ats2
      &&& binding_bv_eq x1 x2
      &&& term_eq ty1 ty2
      &&& term_eq e1 e2
@@ -557,12 +573,12 @@ let rec faithful_lemma (t1 t2 : term) =
 
   | Tv_Match sc1 o1 brs1, Tv_Match sc2 o2 brs2 ->
     assume ((term_eq sc1 sc2
-     &&& opt_eq match_returns_ascription_eq o1 o2
-     &&& list_eq br_eq brs1 brs2) == term_eq t1 t2); // #2908
-    assert_norm (faithful t1 ==> allP0 faithful_branch brs1); // #2908
-    assert_norm (faithful t2 ==> allP0 faithful_branch brs2); // #2908
+     &&& opt_dec_eq t1 t2 match_returns_ascription_eq o1 o2
+     &&& list_dec_eq t1 t2 br_eq brs1 brs2) == term_eq t1 t2); // #2908
+    assert_norm (faithful t1 ==> allP t1 faithful_branch brs1); // #2908
+    assert_norm (faithful t2 ==> allP t2 faithful_branch brs2); // #2908
     faithful_lemma sc1 sc2;
-    faithful_lemma_branches brs1 brs2;
+    faithful_lemma_branches t1 t2 brs1 brs2;
     ()
 
   | Tv_AscribedT e1 t1 tacopt1 eq1, Tv_AscribedT e2 t2 tacopt2 eq2 ->
@@ -586,29 +602,40 @@ and faithful_lemma_pattern (p1 p2 : pattern) : Lemma (requires faithful_pattern 
   | Pat_Var v1 _, Pat_Var v2 _ -> ()
   | Pat_Constant c1, Pat_Constant c2 -> ()
   | Pat_Dot_Term (Some t1), Pat_Dot_Term (Some t2) -> faithful_lemma t1 t2
-  | Pat_Cons f1 us1 args1, Pat_Cons f2 us2 args2 ->
-    assert_norm (faithful_pattern p1 ==> allP0 faithful_pattern_arg args1); // #2908
-    assert_norm (faithful_pattern p2 ==> allP0 faithful_pattern_arg args2); // #2908
-    assume (defined (opt_eq (list_eq univ_eq) us1 us2));
-    (* currently broken due to termination refinements *)
-    //(match us1, us2 with | Some us1, Some us2 ->
-    //  assume (us1 << p1);
-    //  assume (us2 << p2);
-    //  univ_faithful_lemma_list p1 p2 us1 us2 | _ -> ());
-    faithful_lemma_pattern_args args1 args2;
+  | Pat_Cons f1 uso1 args1, Pat_Cons f2 uso2 args2 ->
+    assert_norm (faithful_pattern p1 ==> allP p1 faithful_pattern_arg args1); // #2908
+    assert_norm (faithful_pattern p2 ==> allP p2 faithful_pattern_arg args2); // #2908
+    let aux : squash (defined (opt_dec_eq p1 p2 (list_dec_eq p1 p2 univ_eq) uso1 uso2)) =
+      match uso1, uso2 with
+      | Some us1, Some us2 ->
+        univ_faithful_lemma_list p1 p2 us1 us2
+      | _ -> ()
+    in
+    assert (defined (opt_dec_eq p1 p2 (list_dec_eq p1 p2 univ_eq) uso1 uso2));
+    faithful_lemma_pattern_args p1 p2 args1 args2;
     assert_norm (
         (fv_eq f1 f2
-        &&& opt_eq (list_eq univ_eq) us1 us2
-        &&& list_eq pat_arg_eq args1 args2) == pat_eq p1 p2)
+        &&& opt_dec_eq p1 p2 (list_dec_eq p1 p2 univ_eq) uso1 uso2
+        &&& list_dec_eq p1 p2 pat_arg_eq args1 args2) == pat_eq p1 p2)
 
   | _ -> ()
 
-and faithful_lemma_pattern_arg (pb1 pb2 : pattern & bool) : Lemma (requires faithful_pattern_arg pb1 /\ faithful_pattern_arg pb2) (ensures defined (pat_arg_eq pb1 pb2)) =
+and faithful_lemma_pattern_arg (pb1 pb2 : pattern & bool)
+  : Lemma (requires faithful_pattern_arg pb1 /\ faithful_pattern_arg pb2)
+          (ensures defined (pat_arg_eq pb1 pb2))
+  =
   let (p1, _) = pb1 in
   let (p2, _) = pb2 in
   faithful_lemma_pattern p1 p2
 
-and faithful_lemma_pattern_args (pats1 pats2 : list (pattern & bool)) : Lemma (requires allP0 faithful_pattern_arg pats1 /\ allP0 faithful_pattern_arg pats2) (ensures defined (list_eq pat_arg_eq pats1 pats2)) =
+and faithful_lemma_pattern_args #b
+  (top1 top2 : b)
+  (pats1 : list (pattern & bool){pats1 << top1})
+  (pats2 : list (pattern & bool){pats2 << top2})
+  : Lemma (requires allP top1 faithful_pattern_arg pats1 /\ allP top2 faithful_pattern_arg pats2)
+          (ensures defined (list_dec_eq top1 top2 pat_arg_eq pats1 pats2))
+          (decreases pats1)
+  =
   introduce forall x y. L.memP x pats1 /\ L.memP y pats2 ==> defined (pat_arg_eq x y) with
    (introduce forall y. L.memP x pats1 /\ L.memP y pats2 ==> defined (pat_arg_eq x y) with
     (introduce (L.memP x pats1 /\ L.memP y pats2) ==> (defined (pat_arg_eq x y)) with h. (
@@ -617,13 +644,19 @@ and faithful_lemma_pattern_args (pats1 pats2 : list (pattern & bool)) : Lemma (r
     )
    )
   ;
-  defined_list pat_arg_eq pats1 pats2
+  defined_list_dec top1 top2 pat_arg_eq pats1 pats2
 
 and faithful_lemma_branch (br1 br2 : branch) : Lemma (requires faithful_branch br1 /\ faithful_branch br2) (ensures defined (br_eq br1 br2)) =
   faithful_lemma_pattern (fst br1) (fst br2);
   faithful_lemma (snd br1) (snd br2)
 
-and faithful_lemma_branches (brs1 brs2 : list branch) : Lemma (requires allP0 faithful_branch brs1 /\ allP0 faithful_branch brs2) (ensures defined (list_eq br_eq brs1 brs2)) =
+and faithful_lemma_branches #b (top1 top2 : b)
+  (brs1 : list branch{brs1 << top1})
+  (brs2 : list branch{brs2 << top2})
+  : Lemma (requires allP top1 faithful_branch brs1 /\ allP top2 faithful_branch brs2)
+          (ensures defined (list_dec_eq top1 top2 br_eq brs1 brs2))
+          (decreases brs1)
+  =
   introduce forall x y. L.memP x brs1 /\ L.memP y brs2 ==> defined (br_eq x y) with
    (introduce forall y. L.memP x brs1 /\ L.memP y brs2 ==> defined (br_eq x y) with
     (introduce (L.memP x brs1 /\ L.memP y brs2) ==> (defined (br_eq x y)) with h. (
@@ -632,7 +665,7 @@ and faithful_lemma_branches (brs1 brs2 : list branch) : Lemma (requires allP0 fa
     )
    )
   ;
-  defined_list br_eq brs1 brs2
+  defined_list_dec top1 top2 br_eq brs1 brs2
 
 and faithful_lemma_arg (a1 a2 : argv) : Lemma (requires faithful_arg a1 /\ faithful_arg a2) (ensures defined (arg_eq a1 a2)) =
   faithful_lemma (fst a1) (fst a2);
@@ -643,12 +676,12 @@ and faithful_lemma_binder (b1 b2 : binder) : Lemma (requires faithful_binder b1 
   let bv2 = inspect_binder b2 in
   faithful_lemma_qual bv1.binder_qual bv2.binder_qual;
   faithful_lemma bv1.binder_sort bv2.binder_sort;
-  faithful_lemma_attrs bv1.binder_attrs bv2.binder_attrs;
+  faithful_lemma_attrs_dec b1 b2 bv1.binder_attrs bv2.binder_attrs;
   assert_norm (
       (binding_bv_eq bv1.binder_bv bv2.binder_bv
        &&& term_eq bv1.binder_sort bv2.binder_sort
        &&& aqual_eq bv1.binder_qual bv2.binder_qual
-       &&& list_eq term_eq bv1.binder_attrs bv2.binder_attrs) == binder_eq b1 b2);
+       &&& list_dec_eq b1 b2 term_eq bv1.binder_attrs bv2.binder_attrs) == binder_eq b1 b2);
   ()
 
 and faithful_lemma_qual (q1 q2 : aqualv) : Lemma (requires faithful_qual q1 /\ faithful_qual q2) (ensures defined (aqual_eq q1 q2)) =
@@ -656,7 +689,13 @@ and faithful_lemma_qual (q1 q2 : aqualv) : Lemma (requires faithful_qual q1 /\ f
   | Q_Meta t1, Q_Meta t2 -> faithful_lemma t1 t2
   | _ -> ()
 
-and faithful_lemma_attrs (at1 at2 : list term) : Lemma (requires faithful_attrs at1 /\ faithful_attrs at2) (ensures defined (list_eq term_eq at1 at2)) =
+and faithful_lemma_attrs_dec #b (top1 top2 : b)
+  (at1 : list term{at1 << top1})
+  (at2 : list term{at2 << top2})
+  : Lemma (requires faithful_attrs at1 /\ faithful_attrs at2)
+          (ensures defined (list_dec_eq top1 top2 term_eq at1 at2))
+          (decreases at1)
+  =
   // TODO: factor out
   introduce forall x y. L.memP x at1 /\ L.memP y at2 ==> defined (term_eq x y) with
    (introduce forall y. L.memP x at1 /\ L.memP y at2 ==> defined (term_eq x y) with
@@ -666,7 +705,7 @@ and faithful_lemma_attrs (at1 at2 : list term) : Lemma (requires faithful_attrs 
     )
    )
   ;
-  defined_list term_eq at1 at2
+  defined_list_dec top1 top2 term_eq at1 at2
 
 and faithful_lemma_comp (c1 c2 : comp) : Lemma (requires faithful_comp c1 /\ faithful_comp c2) (ensures defined (comp_eq c1 c2)) =
   match inspect_comp c1, inspect_comp c2 with
@@ -677,9 +716,7 @@ and faithful_lemma_comp (c1 c2 : comp) : Lemma (requires faithful_comp c1 /\ fai
     faithful_lemma post1 post2;
     faithful_lemma pat1 pat2
   | C_Eff us1 e1 r1 args1 dec1, C_Eff us2 e2 r2 args2 dec2 ->
-    // FIXME, termination
-    assume (defined (list_eq univ_eq us1 us2));
-    //univ_faithful_lemma_list us1 us2;
+    univ_faithful_lemma_list c1 c2 us1 us2;
     faithful_lemma r1 r2;
     introduce forall x y. L.memP x args1 /\ L.memP y args2 ==> defined (arg_eq x y) with
      (introduce forall y. L.memP x args1 /\ L.memP y args2 ==> defined (arg_eq x y) with
@@ -689,7 +726,7 @@ and faithful_lemma_comp (c1 c2 : comp) : Lemma (requires faithful_comp c1 /\ fai
       )
      )
     ;
-    defined_list arg_eq args1 args2;
+    defined_list_dec c1 c2 arg_eq args1 args2;
     introduce forall x y. L.memP x dec1 /\ L.memP y dec2 ==> defined (term_eq x y) with
      (introduce forall y. L.memP x dec1 /\ L.memP y dec2 ==> defined (term_eq x y) with
       (introduce (L.memP x dec1 /\ L.memP y dec2) ==> (defined (term_eq x y)) with h. (
@@ -698,13 +735,13 @@ and faithful_lemma_comp (c1 c2 : comp) : Lemma (requires faithful_comp c1 /\ fai
       )
      )
     ;
-    defined_list term_eq dec1 dec2;
+    defined_list_dec c1 c2 term_eq dec1 dec2;
     assume (
-       (list_eq univ_eq us1 us2
+       (list_dec_eq c1 c2 univ_eq us1 us2
         &&& eq_eq e1 e2
         &&& term_eq r1 r2
-        &&& list_eq arg_eq args1 args2
-        &&& list_eq term_eq dec1 dec2) == comp_eq c1 c2); // #2908
+        &&& list_dec_eq c1 c2 arg_eq args1 args2
+        &&& list_dec_eq c1 c2 term_eq dec1 dec2) == comp_eq c1 c2); // #2908
     ()
   | _ -> ()
 #pop-options
